### Test Case 1

Input

```
7
1 3 7
2 3 7
3 1 2 4 5
4 3  6
5 3 6
6 4 5
7 1 2
1 5 2
2 8 6
3 5 8 10 15
4 10 2
5 15 6
6 2 6
7 2 6
3
```


Output

```
5 8 0 10 15 12 7
```

Explanation for output

```
 (3-1) = 5(3-1)
 (3-2) = 8(3-2)
 (3-3) = 0
 (3-4) = 10(3-4)
 (3-5) = 15(3-5)
 (3-6) = 10(3-4) +2(4-6)
 (3-7) = 5(3-1) + 2(1-7)
```

### Test Case 2

Input

```
6
1 2 3 4
2 1 3
3 1 2 4 6
4 1 3 5 6
5 4 6
6 3 4 5
1 2 5 9
2 2 4
3 5 4 3 6
4 9 3 7 8
5 7 1
6 6 8 1
4
```


Output

```
8 7 3 0 7 8
```

Explanation for output

```
(4-1) = 3(4-3) +5(3-1)
(4-2) = 3(4-3) + 4(3-2)
(4-3) = 3(4-3)
(4-4) =0
(4-5) = 7(4-5)
(4-6) = 8(4-6)

```


### Test Case 3

Input

```
5
1 2
2 1 3 4
3 2 4 5
4 2 3 5
5 3 4
1 2 
2 2 5 4
3 5 3 4
4 4 3 2
5 4 2
5
```


Output

```
8 6 4 2 0
```

Explanation for output

```
(5-1) = 2(5-4) + 4(4-2) +2(2-1)
(5-2) = 2(5-4) + 4(4-2)
(5-3) = 4(5-3)
(5-4) = 2(5-4)
(5-5) = 0
```


### Test Case 4

Input

```
5
1 2 3 4 5
2 1 3 4
3 1 2 4
4 1 2 3 5
5 1 4
1 1 2 1 4
2 1 2 3
3 2 2 3
4 1 3 3 4
5 4 4
2
```


Output

```
1 0 2 2 5
```

Explanation for output

```
(2-1) = 1(2-1)
(2-2) = 0
(2-3) = 2(2-3)
(2-4) = 1(2-1) + 1(1-4)
(2-5) = 5(2-5)

```
